====
Sumz
====

Overview
--------

The sumz function returns the sum of values returned from a z-query when the z-query is a string. If the z-query is a proper z-query expression then the sum function should be used.
 
Syntax
------

``=sumz(Z-query-string)``


Arguments
---------

====================  ===========================================================================
Argument              Description
====================  ===========================================================================
``z-query-string``    A z-query string.
====================  ===========================================================================

Example
-------

See section hypernumbers database queries
